remove listR

Deque.thy
@@ -12,32 +12,27 @@ fixes deqL :: "'q \<Rightarrow> 'q"
 fixes deqR :: "'q \<Rightarrow> 'q"
 fixes is_empty :: "'q \<Rightarrow> bool"
 fixes listL :: "'q \<Rightarrow> 'a list"
-fixes listR :: "'q \<Rightarrow> 'a list"
 fixes invar :: "'q \<Rightarrow> bool"
 
-assumes listL_empty:
+assumes list_empty:
  "listL empty = []"
-assumes listR_empty:
- "listR empty = []"
 
 assumes list_enqL:   
  "invar q \<Longrightarrow> listL(enqL x q) = x # listL q"
-assumes list_enqueueRight:  
- "invar q \<Longrightarrow> listR(enqR x q) = x # listR q"
-assumes list_dequeueLeft:   
+assumes list_enqR:  
+ "invar q \<Longrightarrow> rev (listL (enqR x q)) = x # rev (listL q)"
+assumes list_deqL:   
  "\<lbrakk>invar q; \<not> listL q = []\<rbrakk> \<Longrightarrow> listL(deqL q) = tl(listL q)"
-assumes list_dequeueRight: 
- "\<lbrakk>invar q; \<not> listR q = []\<rbrakk> \<Longrightarrow> listR(deqR q) = tl(listR q)"
+assumes list_deqR: 
+ "\<lbrakk>invar q; \<not> rev (listL q) = []\<rbrakk> \<Longrightarrow> rev (listL (deqR q)) = tl (rev (listL q))"
 
 assumes list_firstL:
  "\<lbrakk>invar q; \<not> listL q = []\<rbrakk> \<Longrightarrow> firstL q = hd(listL q)"
 assumes list_firstR:
- "\<lbrakk>invar q; \<not> listR q = []\<rbrakk> \<Longrightarrow> firstR q = hd(listR q)"
+ "\<lbrakk>invar q; \<not> rev (listL q) = []\<rbrakk> \<Longrightarrow> firstR q = hd(rev(listL q))"
 
-assumes listL_is_empty:  
+assumes list_is_empty:  
  "invar q \<Longrightarrow> is_empty q = (listL q = [])"
-assumes listRight_isEmpty:
- "invar q \<Longrightarrow> is_empty q = (listR q = [])"
 
 assumes invar_empty: 
  "invar empty"
@@ -50,7 +45,13 @@ assumes invar_deqL:
  "\<lbrakk>invar q; \<not> is_empty q\<rbrakk>  \<Longrightarrow> invar(deqL q)"
 assumes invar_deqR: 
  "\<lbrakk>invar q; \<not> is_empty q\<rbrakk>  \<Longrightarrow> invar(deqR q)"
-assumes listL_listR: 
- "invar q \<Longrightarrow> listL q = rev (listR q)"
+begin
+
+abbreviation listR :: "'q \<Rightarrow> 'a list" where
+  "listR deque \<equiv> rev (listL deque)"
+
+end
+
+
 
 end
