Transforming.thy
@@ -1,20 +1,16 @@
-theory Transformation 
+theory Transforming 
   imports States
 begin
 
-datatype 'a transformation =
+datatype 'a states =
    Left "'a Small.state" "'a Big.state"
  | Right "'a Big.state" "'a Small.state"
 
-fun listL :: "'a transformation \<Rightarrow> 'a list" where
+fun listL :: "'a states \<Rightarrow> 'a list" where
   "listL (Left small big)  = States.list_small_first (big, small)"
 | "listL (Right big small) = States.list_big_first (big, small)"
- 
-fun listR :: "'a transformation \<Rightarrow> 'a list" where
-  "listR (Left small big)  = States.list_big_first (big, small)"
-| "listR (Right big small) = States.list_small_first (big, small)"
 
-fun step :: "'a transformation \<Rightarrow> 'a transformation" where
+fun step :: "'a states \<Rightarrow> 'a states" where
   "step (Left small big) = (case States.step (big, small) of (big, small) \<Rightarrow> Left small big)"
 | "step (Right big small) = (case States.step (big, small) of (big, small) \<Rightarrow> Right big small)"  
 
@@ -24,20 +20,20 @@ abbreviation four_steps where
 abbreviation six_steps where
   "six_steps \<equiv> step^^6"
 
-instantiation transformation::(type) invar
+instantiation states::(type) invar
 begin
 
-fun invar :: "'a transformation \<Rightarrow> bool" where
+fun invar :: "'a states \<Rightarrow> bool" where
   "invar (Left small big)  \<longleftrightarrow> States.invar (big, small)"
 | "invar (Right big small) \<longleftrightarrow> States.invar (big, small)"
 
 instance..
 end
 
-instantiation transformation::(type) emptyable
+instantiation states::(type) emptyable
 begin
 
-fun is_empty :: "'a transformation \<Rightarrow> bool" where
+fun is_empty :: "'a states \<Rightarrow> bool" where
   "is_empty (Left small big)  \<longleftrightarrow> States.is_empty (big, small)"
 | "is_empty (Right big small) \<longleftrightarrow> States.is_empty (big, small)"
 
@@ -48,11 +44,11 @@ fun remaining_steps where
   "remaining_steps (Left small big) = States.remaining_steps (big, small)"
 | "remaining_steps (Right big small) = States.remaining_steps (big, small)"
 
-fun size_ok :: "'a transformation \<Rightarrow> bool" where
+fun size_ok :: "'a states \<Rightarrow> bool" where
   "size_ok (Left small big) = States.size_ok (big, small)"
 | "size_ok (Right big small) = States.size_ok (big, small)"
 
-fun size_ok' :: "'a transformation \<Rightarrow> nat \<Rightarrow> bool" where
+fun size_ok' :: "'a states \<Rightarrow> nat \<Rightarrow> bool" where
   "size_ok' (Left small big) steps = States.size_ok' (big, small) steps"
 | "size_ok' (Right big small) steps = States.size_ok' (big, small) steps"
 
