RealTimeDeque_Enqueue.thy
@@ -1,5 +1,5 @@
 theory RealTimeDeque_Enqueue
-  imports Deque RealTimeDeque Transformation_Proof
+  imports Deque RealTimeDeque Transforming_Proof
 begin
 
 lemma helper: "\<lbrakk>\<not> leftLength \<le> 3 * Stack.size right; idle.Idle left leftLength = Idle.push x left'; Idle.invar left'; rightLength = Stack.size right;
@@ -50,7 +50,7 @@ next
         by (metis Idle.list.simps Idle_Proof.push_list)+
     next
       case False
-      let ?transformation = "(Right 
+      let ?states = "(Right 
           (Reverse (Current [] 0 left (leftLength - Suc (Stack.size right))) left [] (leftLength - Suc (Stack.size right)))
           (Reverse1 (Current [] 0 right (Suc (2 * Stack.size right))) right []))"
 
@@ -62,7 +62,7 @@ next
           by auto
       qed
 
-      from False have invar: "Transformation.invar ?transformation"
+      from False have invar: "Transforming.invar ?states"
         apply(auto)
         apply(auto simp: reverseN_take popN_drop left_not_empty)
         apply (metis Idle.invar.simps Idle_Proof.invar_push diff_le_self)
@@ -70,12 +70,12 @@ next
         apply (smt (verit) popN_drop append_take_drop_id diff_is_0_eq helper left_not_empty length_rev rev_append rev_rev_ident Stack_Proof.size_list_length take_all_iff)
         by (metis Idle.invar.simps Idle_Proof.invar_push add_Suc_right diff_add_inverse)
      
-      then have "Transformation.listL ?transformation = x # Idle.list left' @ rev (Stack.list right)"
+      then have "Transforming.listL ?states = x # Idle.list left' @ rev (Stack.list right)"
         apply(auto simp: reverseN_take)
         by (metis (no_types, lifting) Idle.hyps Idle.list.simps Idle_Proof.push_list append_Cons append_assoc rev_append rev_swap)
 
       with invar have 
-         "Transformation.listL (six_steps ?transformation) = x # Idle.list left' @ rev (Stack.list right)"
+         "Transforming.listL (six_steps ?states) = x # Idle.list left' @ rev (Stack.list right)"
         by (auto simp: n_steps)
 
       with False show ?case
@@ -86,47 +86,47 @@ next
   case (6 x left right)
   let ?newLeft = "Small.push x left"
   let ?newTransfomation = "Left ?newLeft right"
-  let ?steppedTransformation = "four_steps ?newTransfomation"
+  let ?steppedTransforming = "four_steps ?newTransfomation"
 
-  from 6 have invar: "Transformation.invar ?newTransfomation"
-    by (meson invar.simps(6) Transformation.invar.simps(1) invar_push_small)
+  from 6 have invar: "Transforming.invar ?newTransfomation"
+    by (meson invar.simps(6) Transforming.invar.simps(1) invar_push_small)
 
-  then have list: "Transformation.listL ?newTransfomation = x # Small.list_current left @ rev (Big.list_current right)"
+  then have list: "Transforming.listL ?newTransfomation = x # Small.list_current left @ rev (Big.list_current right)"
     by(auto simp: push_small push_list_current)
                         
-  from invar have four_steps: "Transformation.invar ?steppedTransformation"
+  from invar have four_steps: "Transforming.invar ?steppedTransforming"
     using invar_n_steps by blast
 
-  then have "Transformation.listL ?steppedTransformation = x # Small.list_current left @ rev (Big.list_current right)"
+  then have "Transforming.listL ?steppedTransforming = x # Small.list_current left @ rev (Big.list_current right)"
     using n_steps invar list by fastforce
 
   with 6 show ?case
-    by(auto simp: Let_def split: transformation.splits state_splits)
+    by(auto simp: Let_def split: states.splits state_splits)
 next
   case (7 x left right)
 
   let ?newLeft = "Big.push x left"
   let ?newTransfomation = "Right ?newLeft right"
-  let ?steppedTransformation = "four_steps ?newTransfomation"
+  let ?steppedTransforming = "four_steps ?newTransfomation"
 
-  from 7 have invar: "Transformation.invar ?newTransfomation"
-    by (meson RealTimeDeque.invar.simps Transformation.invar.simps invar_push_big)
+  from 7 have invar: "Transforming.invar ?newTransfomation"
+    by (meson RealTimeDeque.invar.simps Transforming.invar.simps invar_push_big)
 
-  then have listR: "Transformation.listR ?newTransfomation = Small.list_current right @ rev (Big.list_current (Big.push x left))"
+  then have "Transforming.listL ?newTransfomation = list_big_first (Big.push x left, right)"
     by auto
 
-  with invar have listL: "Transformation.listL ?newTransfomation = x # Big.list_current left @ rev (Small.list_current right)"
+  with invar have listL: "Transforming.listL ?newTransfomation = x # Big.list_current left @ rev (Small.list_current right)"
     apply(auto simp: push_big split: prod.splits)
     by (metis Big_Proof.push_list_current append_Cons rev_append rev_rev_ident)
   
-  from invar have four_steps: "Transformation.invar ?steppedTransformation"
+  from invar have four_steps: "Transforming.invar ?steppedTransforming"
     using invar_n_steps by blast
 
-  then have "Transformation.listL ?steppedTransformation = x # Big.list_current left @ rev (Small.list_current right)"
+  then have "Transforming.listL ?steppedTransforming = x # Big.list_current left @ rev (Small.list_current right)"
     using n_steps invar listL by fastforce
 
   with 7 show ?case 
-    apply(auto simp: Let_def split: transformation.split prod.split Big.state.split Common.state.split Small.state.split)
+    apply(auto simp: Let_def split: states.split prod.split Big.state.split Common.state.split Small.state.split)
     by (metis rev_append rev_rev_ident)+
 qed
 
@@ -203,7 +203,7 @@ proof(induction n arbitrary: small big)
 next
   case (Suc n)
   then show ?case 
-    by (metis (no_types, lifting) Transformation.step.simps(1) comp_def funpow_Suc_right prod.case_eq_if) 
+    by (metis (no_types, lifting) Transforming.step.simps(1) comp_def funpow_Suc_right prod.case_eq_if) 
 qed
 
 lemma step_same_right: "case step (Right big small) of Right _ _ \<Rightarrow> True | _ \<Rightarrow> False"
@@ -216,24 +216,24 @@ proof(induction n arbitrary: small big)
 next
   case (Suc n)
   then show ?case 
-    by (metis (no_types, lifting) Transformation.step.simps(2) comp_def funpow_Suc_right prod.case_eq_if) 
+    by (metis (no_types, lifting) Transforming.step.simps(2) comp_def funpow_Suc_right prod.case_eq_if) 
 qed
 
-lemma remaining_steps_not_idle: "Transformation.invar transformation \<Longrightarrow> remaining_steps transformation > 0 \<longleftrightarrow> (
-    case transformation of 
+lemma remaining_steps_not_idle: "Transforming.invar states \<Longrightarrow> remaining_steps states > 0 \<longleftrightarrow> (
+    case states of 
       Left (Small.Common (Common.Idle _ _)) (Big.Common (Common.Idle _ _))  \<Rightarrow> False 
     | Right (Big.Common (Common.Idle _ _)) (Small.Common (Common.Idle _ _))  \<Rightarrow> False 
     | _ \<Rightarrow> True) "
-  apply(induction transformation)
+  apply(induction states)
   by(auto split: Big.state.splits Small.state.splits Common.state.splits current.splits)
 
-lemma remaining_steps_left_idle: "Transformation.invar (Left small big) \<Longrightarrow> remaining_steps (Left small big) = 0 \<longleftrightarrow> (
+lemma remaining_steps_left_idle: "Transforming.invar (Left small big) \<Longrightarrow> remaining_steps (Left small big) = 0 \<longleftrightarrow> (
     case (Left small big) of 
       Left (Small.Common (Common.Idle _ _)) (Big.Common (Common.Idle _ _))  \<Rightarrow> True 
     | _ \<Rightarrow> False) "
   by(auto split: Big.state.splits Small.state.splits Common.state.splits current.splits)
 
-lemma remaining_steps_right_idle: "Transformation.invar (Right big small) \<Longrightarrow> remaining_steps (Right big small) = 0 \<longleftrightarrow> (
+lemma remaining_steps_right_idle: "Transforming.invar (Right big small) \<Longrightarrow> remaining_steps (Right big small) = 0 \<longleftrightarrow> (
     case (Right big small) of 
       Right (Big.Common (Common.Idle _ _)) (Small.Common (Common.Idle _ _))  \<Rightarrow> True 
     | _ \<Rightarrow> False) "
@@ -272,7 +272,7 @@ next
       
       let ?newLeftLength = "leftLength - (Stack.size right) - 1"
       let ?newRightLength = "Suc (2 * Stack.size right)"
-      let ?transformation = "(Right 
+      let ?states = "(Right 
           (Reverse (Current [] 0 left ?newLeftLength) left [] ?newLeftLength)
           (Reverse1 (Current [] 0 right ?newRightLength) right []))"
 
@@ -292,30 +292,30 @@ next
         apply auto 
         by (metis Idle.size.simps Idle_Proof.size_push leftLength)    
 
-      from False have remaining_steps: "6 < Transformation.remaining_steps ?transformation"
+      from False have remaining_steps: "6 < Transforming.remaining_steps ?states"
         apply(auto simp: max_def)
         by (smt (z3) add.commute add_2_eq_Suc' diff_add_inverse2 diff_is_0_eq le_less_Suc_eq length_greater_0_conv leftLength mult_Suc Stack_Proof.size_not_empty not_le not_less_eq numeral_3_eq_3 numeral_Bit0 Stack_Proof.size_list_length old_size)
         
-      from False have invar: "Transformation.invar ?transformation"
+      from False have invar: "Transforming.invar ?states"
         apply(auto simp: Stack_Proof.size_list_length popN_drop left_not_empty)
            apply (metis Idle.invar.simps Idle_Proof.invar_push diff_le_self Stack_Proof.size_list_length)
           apply (simp add: reverseN_take)
         apply (smt (verit, best) popN_drop Suc_leI diff_add_inverse diff_add_inverse2 diff_diff_left helper4 le_eq_less_or_eq left_not_empty length_drop mult_Suc numeral_3_eq_3 plus_1_eq_Suc reverseN_reverseN Stack_Proof.size_list_length old_size)
         by (metis Idle.invar.simps Idle_Proof.invar_push add_Suc_right diff_add_inverse Stack_Proof.size_list_length)
 
-      with remaining_steps have "5 < Transformation.remaining_steps (step ?transformation)"
-        using remaining_steps_decline_3[of ?transformation 5] by auto
+      with remaining_steps have "5 < Transforming.remaining_steps (step ?states)"
+        using remaining_steps_decline_3[of ?states 5] by auto
 
-      with invar have "4 < Transformation.remaining_steps ((step ^^ 2) ?transformation)"
-        using invar_n_steps invar_step remaining_steps_decline_4[of ?transformation 4 1]
+      with invar have "4 < Transforming.remaining_steps ((step ^^ 2) ?states)"
+        using invar_n_steps invar_step remaining_steps_decline_4[of ?states 4 1]
         by (smt (z3) add.commute add_Suc_right funpow_0 numeral_2_eq_2 numeral_3_eq_3 numeral_Bit0 remaining_steps remaining_steps_decline_4)
 
-      with remaining_steps have remaining_steps_end: "0 < Transformation.remaining_steps (six_steps ?transformation)"
-        using remaining_steps_decline_4[of ?transformation 5 5] 
+      with remaining_steps have remaining_steps_end: "0 < Transforming.remaining_steps (six_steps ?states)"
+        using remaining_steps_decline_4[of ?states 5 5] 
         by (smt (z3) One_nat_def Suc_eq_plus1 add_Suc_right invar numeral_2_eq_2 numeral_3_eq_3 numeral_Bit0 remaining_steps_decline_4)
 
  
-      from False left_not_empty have size_ok: "size_ok' ?transformation (remaining_steps ?transformation - 6)"
+      from False left_not_empty have size_ok: "size_ok' ?states (remaining_steps ?states - 6)"
         apply(auto simp: max_def old_size leftLength)
         subgoal
           proof(induction "Stack.size left + Stack.size right \<le> 4")
@@ -335,14 +335,14 @@ next
               calculation_helper
         by auto
 
-      then have "size_ok' (six_steps ?transformation) (remaining_steps (six_steps ?transformation))"
+      then have "size_ok' (six_steps ?states) (remaining_steps (six_steps ?states))"
         using size_ok_steps invar remaining_steps by blast
 
-      then have six_steps_size_ok: "size_ok (six_steps ?transformation)"
+      then have six_steps_size_ok: "size_ok (six_steps ?states)"
         using size_ok'_size_ok
         using n_steps_size_ok size_ok by blast
 
-     from invar have "Transformation.invar (six_steps ?transformation)"
+     from invar have "Transforming.invar (six_steps ?states)"
        using invar_n_steps by blast
 
       with False six_steps_size_ok show ?case
@@ -354,15 +354,15 @@ next
   case (6 x left right)
   let ?newLeft = "Small.push x left"
   let ?newTransfomation = "Left ?newLeft right"
-  let ?steppedTransformation = "four_steps ?newTransfomation"
+  let ?steppedTransforming = "four_steps ?newTransfomation"
 
   have start_size_ok: "size_ok (Left left right)"
     using "6.prems" invar.simps(6) by blast
 
-  from 6 have invar: "Transformation.invar ?newTransfomation"
-    by (meson invar.simps(6) Transformation.invar.simps(1) invar_push_small)
+  from 6 have invar: "Transforming.invar ?newTransfomation"
+    by (meson invar.simps(6) Transforming.invar.simps(1) invar_push_small)
 
-  then have invar_four_steps: "Transformation.invar (four_steps ?newTransfomation)"
+  then have invar_four_steps: "Transforming.invar (four_steps ?newTransfomation)"
     using invar_n_steps by blast
 
   with 6 show ?case
@@ -373,33 +373,33 @@ next
     from True have states_size_ok: "States.size_ok (right, left)" by auto
     
     from True have "remaining_steps ?newTransfomation > 4"
-      by (metis Transformation.remaining_steps.simps(1) remaining_steps_push_small states_invar)
+      by (metis Transforming.remaining_steps.simps(1) remaining_steps_push_small states_invar)
 
-    then have remaining_steps: "remaining_steps ?steppedTransformation > 0"
+    then have remaining_steps: "remaining_steps ?steppedTransforming > 0"
       by (metis One_nat_def add_Suc_shift funpow_0 invar numeral_2_eq_2 numeral_Bit0 plus_1_eq_Suc remaining_steps_decline_4)
 
-    from True have size_ok: "size_ok ?steppedTransformation"
+    from True have size_ok: "size_ok ?steppedTransforming"
       using step_4_push_small_size_ok[of right left x] states_invar states_rem states_size_ok size_ok_states_left by auto
 
-    have "case ?steppedTransformation of
+    have "case ?steppedTransforming of
       Left (Small.state.Common (state.Idle _ _)) (Big.state.Common (state.Idle _ _)) \<Rightarrow> False
     | _ \<Rightarrow> True"
-      using step_same_left[of ?newLeft right] remaining_steps_not_idle[of ?steppedTransformation]
-      apply(auto split: prod.splits transformation.splits Small.state.splits Big.state.splits Common.state.splits)
+      using step_same_left[of ?newLeft right] remaining_steps_not_idle[of ?steppedTransforming]
+      apply(auto split: prod.splits states.splits Small.state.splits Big.state.splits Common.state.splits)
       using remaining_steps by auto
 
-    then have "(case ?steppedTransformation of 
+    then have "(case ?steppedTransforming of 
       Left 
         (Small.Common (Common.Idle _ left)) 
         (Big.Common (Common.Idle _ right)) \<Rightarrow> Idle left right
-   | _ \<Rightarrow> Transforming ?steppedTransformation) = Transforming ?steppedTransformation"
-      by(auto split: transformation.splits Small.state.splits Common.state.splits Big.state.splits)
+   | _ \<Rightarrow> Transforming ?steppedTransforming) = Transforming ?steppedTransforming"
+      by(auto split: states.splits Small.state.splits Common.state.splits Big.state.splits)
 
-    with True  have "invar (case ?steppedTransformation of 
+    with True  have "invar (case ?steppedTransforming of 
       Left 
         (Small.Common (Common.Idle _ left)) 
         (Big.Common (Common.Idle _ right)) \<Rightarrow> Idle left right
-   | _ \<Rightarrow> Transforming ?steppedTransformation)"
+   | _ \<Rightarrow> Transforming ?steppedTransforming)"
       by (smt (z3) invar.simps(6) remaining_steps size_ok) 
 
     with True show ?case
@@ -408,13 +408,13 @@ next
   next
     case False
     then have "remaining_steps ?newTransfomation \<le> 4"
-      by (metis invar.simps(6) Transformation.invar.simps(1) Transformation.remaining_steps.simps(1) leI remaining_steps_push_small)
+      by (metis invar.simps(6) Transforming.invar.simps(1) Transforming.remaining_steps.simps(1) leI remaining_steps_push_small)
 
-    with False have remaining_steps: "remaining_steps ?steppedTransformation = 0"
+    with False have remaining_steps: "remaining_steps ?steppedTransforming = 0"
       using invar remaining_steps_decline_5[of ?newTransfomation 4]
       by auto
 
-    obtain steppedL steppedR where stepped: "?steppedTransformation = Left steppedL steppedR"
+    obtain steppedL steppedR where stepped: "?steppedTransforming = Left steppedL steppedR"
       using step_same_left_n[of 4 ?newLeft right]
       by (simp add: case_prod_unfold numeral_Bit0)
 
@@ -427,7 +427,7 @@ next
       Left (Small.state.Common (state.Idle l idleL)) (Big.state.Common (state.Idle r idleR))"
       by(auto split: Small.state.splits Common.state.splits Big.state.splits)
 
-    then have transformation_invar: "Transformation.invar (Left steppedL steppedR)"
+    then have states_invar: "Transforming.invar (Left steppedL steppedR)"
       using False
       using \<open>four_steps (Left (Small.push x left) right) = Left steppedL steppedR\<close>
       by auto
@@ -436,13 +436,13 @@ next
       using invar step_n_left_size_new_big by blast
 
     have left_sizes_1: "Small.size ?newLeft = Suc (Small.size left)"
-      by (meson "6.prems" invar.simps(6) Transformation.invar.simps(1) funpow_0 step_n_push_size_small)
+      by (meson "6.prems" invar.simps(6) Transforming.invar.simps(1) funpow_0 step_n_push_size_small)
 
     with stepped invar_four_steps have left_sizes: "Small.size_new ?newLeft = Small.size_new steppedL"
       using invar step_n_left_size_new_small by blast
 
     then have "0 < Small.size_new left"
-      using "6.prems" invar.simps(6) size_ok.simps(1) Transformation.invar.simps(1) size_ok_size_new_small by blast
+      using "6.prems" invar.simps(6) size_ok.simps(1) Transforming.invar.simps(1) size_ok_size_new_small by blast
 
     then have "0 < Small.size_new ?newLeft"
       using \<open>Small.size (Small.push x left) = Suc (Small.size left)\<close> invar Small_Proof.size_size_new by fastforce
@@ -451,23 +451,23 @@ next
       by (simp add: \<open>Small.size_new (Small.push x left) = Small.size_new steppedL\<close>)
 
     then have "0 < Big.size_new right"
-      using "6.prems" invar.simps(6) size_ok.simps(1) Transformation.invar.simps(1) size_ok_size_new_big by blast
+      using "6.prems" invar.simps(6) size_ok.simps(1) Transforming.invar.simps(1) size_ok_size_new_big by blast
 
     then have right_not_empty: "0 < Big.size_new steppedR"
       by (simp add: \<open>Big.size_new right = Big.size_new steppedR\<close>)
 
     have left_size: "Idle.size idleL = Small.size_new steppedL"
-      using idle transformation_invar by auto
+      using idle states_invar by auto
 
     have right_size: "Idle.size idleR = Big.size_new steppedR"
-      using idle transformation_invar by auto
+      using idle states_invar by auto
 
     have wind2: "Small.size_new left \<le> 3 * Big.size_new right - 1"
       using start_size_ok
       by auto
 
     have "Suc (Small.size_new left) = Small.size_new ?newLeft"
-      by (metis "6.prems" invar.simps(6) Transformation.invar.simps(1) funpow_0 step_n_push_size_new_small)
+      by (metis "6.prems" invar.simps(6) Transforming.invar.simps(1) funpow_0 step_n_push_size_new_small)
 
     with wind2 have "Small.size_new ?newLeft \<le> 3 * Big.size_new right"
       using \<open>0 < Big.size_new right\<close> by linarith
@@ -484,7 +484,7 @@ next
 
     then have "Big.size_new right \<le> 3 * Small.size_new ?newLeft"
       using left_sizes_1
-      by (metis (no_types, opaque_lifting) "6.prems" invar.simps(6) Transformation.invar.simps(1) dual_order.trans funpow_0 le_add2 mult_le_mono2 plus_1_eq_Suc step_n_push_size_new_small)
+      by (metis (no_types, opaque_lifting) "6.prems" invar.simps(6) Transforming.invar.simps(1) dual_order.trans funpow_0 le_add2 mult_le_mono2 plus_1_eq_Suc step_n_push_size_new_small)
 
     then have "Big.size_new right \<le> 3 * Small.size_new steppedL"
       by (simp add: left_sizes)
@@ -492,7 +492,7 @@ next
     then have "Big.size_new steppedR \<le> 3 * Small.size_new steppedL"
       by (simp add: \<open>Big.size_new right = Big.size_new steppedR\<close>)
     
-    with idle transformation_invar T have "invar (Idle idleL idleR)"
+    with idle states_invar T have "invar (Idle idleL idleR)"
       apply auto
       apply (metis Common.size_new.simps(1) Idle.is_empty.elims(2) Idle.size.simps Small.size_new.simps(1) \<open>0 < Small.size_new (Small.push x left)\<close> \<open>Small.size_new (Small.push x left) = Small.size_new steppedL\<close> list.size(3) Stack_Proof.size_list_length Stack_Proof.list_not_empty verit_comp_simplify1(1))
       using right_not_empty Idle_Proof.not_empty by auto
@@ -502,24 +502,24 @@ next
         (Small.Common (Common.Idle _ left)) 
         (Big.Common (Common.Idle _ right)) \<Rightarrow> Idle left right
    | _ \<Rightarrow> Transforming (Left steppedL steppedR))"
-       using Big.state.simps(6) Common.state.simps(6) Small.state.simps(12) idle transformation.inject(1) transformation.simps(5) by auto
+       using Big.state.simps(6) Common.state.simps(6) Small.state.simps(12) idle states.inject(1) states.simps(5) by auto
 
      with False show ?case
-       by (metis \<open>four_steps (transformation.Left (Small.push x left) right) = transformation.Left steppedL steppedR\<close> enqL.simps(6))
+       by (metis \<open>four_steps (states.Left (Small.push x left) right) = states.Left steppedL steppedR\<close> enqL.simps(6))
    qed
 next
   case (7 x left right)
   let ?newLeft = "Big.push x left"
   let ?newTransfomation = "Right ?newLeft right"
-  let ?steppedTransformation = "four_steps ?newTransfomation"
+  let ?steppedTransforming = "four_steps ?newTransfomation"
 
   have start_size_ok: "size_ok (Right left right)"
     using "7.prems" invar.simps(6) by blast
 
-  from 7 have invar: "Transformation.invar ?newTransfomation"
-    by (meson invar.simps(6) Transformation.invar.simps invar_push_big)
+  from 7 have invar: "Transforming.invar ?newTransfomation"
+    by (meson invar.simps(6) Transforming.invar.simps invar_push_big)
 
-  then have invar_four_steps: "Transformation.invar (four_steps ?newTransfomation)"
+  then have invar_four_steps: "Transforming.invar (four_steps ?newTransfomation)"
     using invar_n_steps by blast
 
   with 7 show ?case
@@ -532,32 +532,32 @@ next
     from True have "remaining_steps ?newTransfomation > 4"
       by (metis remaining_steps.simps(2) remaining_steps_push_big states_invar)
 
-    then have remaining_steps: "remaining_steps ?steppedTransformation > 0"
+    then have remaining_steps: "remaining_steps ?steppedTransforming > 0"
       by (metis One_nat_def add_Suc_shift funpow_0 invar numeral_2_eq_2 numeral_Bit0 plus_1_eq_Suc remaining_steps_decline_4)
 
-    from True have size_ok: "size_ok ?steppedTransformation"
+    from True have size_ok: "size_ok ?steppedTransforming"
       using step_4_push_big_size_ok[of left right x] states_invar states_rem states_size_ok size_ok_states_right
       by blast
 
-    have "case ?steppedTransformation of
+    have "case ?steppedTransforming of
       Right (Big.state.Common (state.Idle _ _)) (Small.state.Common (state.Idle _ _)) \<Rightarrow> False
     | _ \<Rightarrow> True"
-      using step_same_right[of ?newLeft right] remaining_steps_not_idle[of ?steppedTransformation]
-      apply(auto split: prod.splits transformation.splits Small.state.splits Big.state.splits Common.state.splits)
+      using step_same_right[of ?newLeft right] remaining_steps_not_idle[of ?steppedTransforming]
+      apply(auto split: prod.splits states.splits Small.state.splits Big.state.splits Common.state.splits)
       using remaining_steps by auto
 
-    then have "(case ?steppedTransformation of 
+    then have "(case ?steppedTransforming of 
       Right 
         (Big.Common (Common.Idle _ left)) 
         (Small.Common (Common.Idle _ right)) \<Rightarrow> Idle left right
-   | _ \<Rightarrow> Transforming ?steppedTransformation) = Transforming ?steppedTransformation"
-      by(auto split: transformation.splits Small.state.splits Common.state.splits Big.state.splits)
+   | _ \<Rightarrow> Transforming ?steppedTransforming) = Transforming ?steppedTransforming"
+      by(auto split: states.splits Small.state.splits Common.state.splits Big.state.splits)
 
-    with True  have "invar (case ?steppedTransformation of 
+    with True  have "invar (case ?steppedTransforming of 
       Right 
         (Big.Common (Common.Idle _ left)) 
         (Small.Common (Common.Idle _ right)) \<Rightarrow> Idle left right
-   | _ \<Rightarrow> Transforming ?steppedTransformation)"
+   | _ \<Rightarrow> Transforming ?steppedTransforming)"
       by (smt (z3) invar.simps(6) remaining_steps size_ok) 
 
     with True show ?case
@@ -566,13 +566,13 @@ next
   next
     case False
     then have "remaining_steps ?newTransfomation \<le> 4"
-      by (metis invar.simps(6) Transformation.invar.simps(2) remaining_steps.simps(2) leI remaining_steps_push_big)
+      by (metis invar.simps(6) Transforming.invar.simps(2) remaining_steps.simps(2) leI remaining_steps_push_big)
 
-    with False have remaining_steps: "remaining_steps ?steppedTransformation = 0"
+    with False have remaining_steps: "remaining_steps ?steppedTransforming = 0"
       using invar remaining_steps_decline_5[of ?newTransfomation 4]
       by auto
 
-    obtain steppedL steppedR where stepped: "?steppedTransformation = Right steppedL steppedR"
+    obtain steppedL steppedR where stepped: "?steppedTransforming = Right steppedL steppedR"
       using step_same_right_n[of 4 ?newLeft right]
       by (simp add: case_prod_unfold numeral_Bit0)
 
@@ -585,7 +585,7 @@ next
       Right (Big.state.Common (state.Idle l idleL)) (Small.state.Common (state.Idle r idleR))"
       by(auto split: Small.state.splits Common.state.splits Big.state.splits)
 
-    then have transformation_invar: "Transformation.invar (Right steppedL steppedR)"
+    then have states_invar: "Transforming.invar (Right steppedL steppedR)"
       using False
       using \<open>four_steps (Right (Big.push x left) right) = Right steppedL steppedR\<close>
       by auto
@@ -600,7 +600,7 @@ next
       using invar step_n_right_size_new_big by blast
 
     then have "0 < Big.size_new left"
-     using "7.prems" invar.simps(6) size_ok.simps(1) Transformation.invar.simps(1) size_ok_size_new_big
+     using "7.prems" invar.simps(6) size_ok.simps(1) Transforming.invar.simps(1) size_ok_size_new_big
      by fastforce
 
     then have "0 < Big.size_new ?newLeft"
@@ -610,17 +610,17 @@ next
       by (simp add: \<open>Big.size_new (Big.push x left) = Big.size_new steppedL\<close>)
 
     then have "0 < Small.size_new right"
-      using "7.prems" invar.simps size_ok.simps Transformation.invar.simps size_ok_size_new_small
+      using "7.prems" invar.simps size_ok.simps Transforming.invar.simps size_ok_size_new_small
       by fastforce
 
     then have right_not_empty: "0 < Small.size_new steppedR"
       by (simp add: \<open>Small.size_new right = Small.size_new steppedR\<close>)
 
     have left_size: "Idle.size idleL = Big.size_new steppedL"
-      using idle transformation_invar by auto
+      using idle states_invar by auto
 
     have right_size: "Idle.size idleR = Small.size_new steppedR"
-      using idle transformation_invar by auto
+      using idle states_invar by auto
 
     have size_ok_2: "Big.size_new left \<le> 3 * Small.size_new right - 1"
       using start_size_ok
@@ -652,7 +652,7 @@ next
     then have "Small.size_new steppedR \<le> 3 * Big.size_new steppedL"
       by (simp add: \<open>Small.size_new right = Small.size_new steppedR\<close>)
     
-    with idle transformation_invar T have "invar (Idle idleL idleR)"
+    with idle states_invar T have "invar (Idle idleL idleR)"
       apply auto
       apply (metis Idle.is_empty.elims(2) Idle.size.simps Stack_Proof.size_empty Suc_neq_Zero \<open>Suc (Big.size_new left) = Big.size_new (Big.push x left)\<close> left_size left_sizes)
       using right_not_empty Idle_Proof.not_empty by auto
@@ -662,7 +662,7 @@ next
         (Big.Common (Common.Idle _ left)) 
         (Small.Common (Common.Idle _ right)) \<Rightarrow> Idle left right
    | _ \<Rightarrow> Transforming (Right steppedL steppedR))"
-       using Big.state.simps(6) Common.state.simps(6) Small.state.simps(12) idle transformation.inject(1) transformation.simps(5) by auto
+       using Big.state.simps(6) Common.state.simps(6) Small.state.simps(12) idle states.inject(1) states.simps(5) by auto
 
      with False show ?case
       by (metis enqL.simps(7) stepped)
