RealTimeDeque_Proof.thy
@@ -1,14 +1,24 @@
 theory RealTimeDeque_Proof
-  imports Deque RealTimeDeque Transformation_Proof RealTimeDeque_Enqueue RealTimeDeque_Dequeue
+  imports Deque RealTimeDeque Transforming_Proof RealTimeDeque_Enqueue RealTimeDeque_Dequeue
 begin
-  
-lemma swap: "invar q \<Longrightarrow> listR (swap q) = listL q"
-  apply(induction q rule: swap.induct)
-  by auto
 
-lemma swap': "invar q \<Longrightarrow> listL (swap q) = listR q"
-  apply(induction q rule: swap.induct)
-  by auto
+lemma list_rev: "as @ rev bs = cs @ rev ds \<Longrightarrow> bs @ rev as  = ds @ rev cs"
+  by (metis rev_append rev_rev_ident)
+
+lemma swap_list: "invar q \<Longrightarrow> listR (swap q) = listL q"
+  apply(induction q)
+  apply auto
+  subgoal for t
+  apply(induction t)
+  apply(auto simp: split: prod.splits)
+  subgoal for big small smallList bigList
+    using list_rev[of bigList smallList "Small.list_current small" "Big.list_current big"]
+    by simp
+  . .
+
+lemma swap_list': "invar q \<Longrightarrow> listL (swap q) = listR q"
+  using swap_list rev_swap
+  by blast
 
 lemma invar_swap: "invar q \<Longrightarrow> invar (swap q)"
   apply(induction q rule: swap.induct)
@@ -77,44 +87,12 @@ next
     apply auto
     using Small_Proof.list_current_size apply force
     apply(auto simp: max_def split: prod.splits Big.state.splits Small.state.splits if_splits)
-    subgoal 
-      by(simp add: Nat.diff_diff_right diff_is_0_eq' list.size(3) min.absorb1 minus_nat.diff_0 mult_is_0 not_numeral_le_zero numeral_2_eq_2 Stack_Proof.size_list_length split: current.splits)
+    apply(simp add: size_list_length split!: current.splits)
     subgoal by(auto split!: current.splits)
     subgoal by(auto split: current.splits)
     subgoal by(auto split: current.splits)
     using size_list_common by auto
 qed
-
-lemma listL_rev_listR: "listL deque = rev (listR deque)"
-proof(induction deque)
-  case Empty
-  then show ?case by auto
-next
-  case (One x)
-  then show ?case by auto
-next
-  case (Two x y)
-  then show ?case by auto
-next
-  case (Three x y z)
-  then show ?case by auto
-next
-  case (Idle left right)
-  then show ?case by auto
-next
-  case (Transforming transformation)
-  then show ?case 
-  proof(induction transformation)
-    case (Left small big)
-    then show ?case 
-      by(auto split: prod.splits)
-  next
-    case (Right big small)
-    then show ?case 
-      by(auto split: prod.splits)
-  qed
-qed
-  
 
 interpretation RealTimeDeque: Deque where
   empty    = empty    and
@@ -126,20 +104,16 @@ interpretation RealTimeDeque: Deque where
   deqR     = deqR     and
   is_empty = is_empty and
   listL    = listL    and
-  listR    = listR    and
   invar    = invar
 proof (standard, goal_cases)
   case 1
   then show ?case by (simp add: empty_def)
 next
-  case 2
-  then show ?case by (simp add: empty_def)
-next
-  case (3 q x)
+  case (2 q x)
   then show ?case
     by(simp add: list_enqL)
 next
-  case (4 q x)
+  case (3 q x)
 
   then have invar_swap: "invar (swap q)"
     by (simp add: invar_swap)
@@ -148,49 +122,49 @@ next
     by (simp add: list_enqL)
 
   then have "listL (enqL x (swap q)) = x # listR q"
-    by(auto simp: 4 swap')
+    by(auto simp: 3 swap_list')
 
   then show ?case
-    using 4 
-    by (simp add: swap invar_enqL invar_swap)
+    using 3
+    by (simp add: swap_list invar_enqL invar_swap)
 next
-  case (5 q)
+  case (4 q)
   then show ?case
     using list_deqL by simp
 next
-  case (6 q)
+  case (5 q)
   then have invar_swap: "invar (swap q)"
     by (simp add: invar_swap)
 
   then have "listL (deqL (swap q)) = tl (listL (swap q))"
-    using 6 list_deqL swap' by fastforce
+    using 5 list_deqL swap_list' by fastforce
 
 
   then have "listL (deqL (swap q)) = tl (listR q)"
-    by (simp add: 6 swap')
+    by (simp add: 5 swap_list')
 
   then have "listR (swap (deqL (swap q))) = tl (listR q)"
-    by (metis "6"(1) "6"(2) is_empty.elims(2) swap invar_deqL invar_swap listL.simps(1) swap')
+    by (metis "5"(1) "5"(2) invar_deqL listL_is_empty invar_swap swap_list swap_list')
 
   then show ?case     
     by(auto split: prod.splits)
 next
-  case (7 q)
+  case (6 q)
   then show ?case
     using list_firstL by simp
 next
-  case (8 q)
+  case (7 q)
 
   then have swap_invar: "invar (swap q)"
     by (simp add: invar_swap)
 
-  from 8 have "listR q = listL (swap q)"
-    by (simp add: swap')
+  from 7 have "listR q = listL (swap q)"
+    by (simp add: swap_list')
 
-  from 8 have "firstR q = firstL (swap q)"
+  from 7 have "firstR q = firstL (swap q)"
     by(auto split: prod.splits)
 
-  from 8 have "listL (swap q) \<noteq> []"
+  from 7 have "listL (swap q) \<noteq> []"
     using \<open>listR q = listL (swap q)\<close> by auto
 
   then have "firstL (swap q) = hd (listL (swap q))"
@@ -199,46 +173,39 @@ next
   then show ?case 
     using \<open>firstR q = firstL (swap q)\<close> \<open>listR q = listL (swap q)\<close> by presburger
 next
-  case (9 q)
+  case (8 q)
   then show ?case using listL_is_empty by auto
 next
-  case (10 q)
+  case (9)
   then show ?case
-    by (simp add: listL_is_empty listL_rev_listR)
-next
-  case 11
-  then show ?case 
     by (simp add: empty_def)
 next
-  case (12 q x)
+  case (10 q x)
   then show ?case by(simp add: invar_enqL)
 next
-  case (13 q x)
+  case (11 q x)
   then have swap: "enqR x q = swap (enqL x (swap q))"
     by simp
 
-  from 13 have "invar (swap (enqL x (swap q)))"
+  from 11 have "invar (swap (enqL x (swap q)))"
     by (simp add: invar_enqL invar_swap)
 
   with swap show ?case 
     by simp
 next
-  case (14 q)
+  case (12 q)
   then show ?case
     using invar_deqL by auto
 next
-  case (15 q)
+  case (13 q)
   then have swap: "deqR q = swap (deqL (swap q))"
     by(auto split: prod.splits)
 
-  from 15 have "invar (swap (deqL (swap q)))"
-    by (metis invar_deqL invar_swap listL_is_empty listL_rev_listR rev.simps(1) swap')
+  from 13 have "invar (swap (deqL (swap q)))"
+    by (metis invar_deqL invar_swap listL_is_empty rev.simps(1) swap_list)
 
   with swap show ?case
     by auto
-next 
-  case (16 q)
-  then show ?case using listL_rev_listR by auto
 qed
 
 end
