Transforming_Proof.thy
@@ -1,9 +1,9 @@
-theory Transformation_Proof
-  imports  Transformation States_Proof
+theory Transforming_Proof
+  imports  Transforming States_Proof
 begin
 
-lemma invar_step: "invar transformation \<Longrightarrow> invar (step transformation)"
-proof(induction transformation rule: step.induct)
+lemma invar_step: "invar states \<Longrightarrow> invar (step states)"
+proof(induction states rule: step.induct)
   case (1 small big)
 
   then have "States.invar (big, small)"
@@ -12,7 +12,7 @@ proof(induction transformation rule: step.induct)
   then have "States.invar (States.step (big, small))"
     using States_Proof.invar_step by blast
 
-  then have "Transformation.invar (case States.step (big, small) of (big, small) \<Rightarrow> Left small big)"
+  then have "Transforming.invar (case States.step (big, small) of (big, small) \<Rightarrow> Left small big)"
     by(auto split: prod.split)
 
   then show ?case by auto
@@ -31,8 +31,8 @@ next
   then show ?case by auto
 qed
 
-lemma step_listL: "invar transformation \<Longrightarrow> listL (step transformation) = listL transformation"
-proof(induction transformation rule: step.induct)
+lemma step_listL: "invar states \<Longrightarrow> listL (step states) = listL states"
+proof(induction states rule: step.induct)
   case (1 small big)
 
   then have "list_small_first (big, small) = Small.list_current small @ rev (Big.list_current big)"
@@ -65,42 +65,42 @@ next
 qed
 
 lemma invar_pop_small_left: "invar (Left small big) \<Longrightarrow> 0 < Small.size small \<Longrightarrow> Small.pop small = (x, small') \<Longrightarrow> invar (Left small' big)"
-  by (meson Transformation.invar.simps(1) invar_pop_small_size)
+  by (meson Transforming.invar.simps(1) invar_pop_small_size)
 
 lemma invar_pop_big_left: "invar (Left small big) \<Longrightarrow> 0 < Big.size big \<Longrightarrow> Big.pop big = (x, big') \<Longrightarrow> invar (Left small big')"
-  by (meson Transformation.invar.simps(1) invar_pop_big_size)
+  by (meson Transforming.invar.simps(1) invar_pop_big_size)
 
 lemma invar_pop_small_right: "invar (Right big small) \<Longrightarrow> 0 < Small.size small \<Longrightarrow> Small.pop small = (x, small') \<Longrightarrow> invar (Right big small')"
-  by (meson Transformation.invar.simps invar_pop_small_size)
+  by (meson Transforming.invar.simps invar_pop_small_size)
 
 lemma invar_pop_big_right: "invar (Right big small) \<Longrightarrow> 0 < Big.size big \<Longrightarrow> Big.pop big = (x, big') \<Longrightarrow> invar (Right big' small)"
-  by (meson Transformation.invar.simps invar_pop_big_size)
+  by (meson Transforming.invar.simps invar_pop_big_size)
 
-lemma n_steps: "invar transformation \<Longrightarrow> listL ((step^^n) transformation) = listL transformation"
-  apply(induction n arbitrary: transformation)
+lemma n_steps: "invar states \<Longrightarrow> listL ((step^^n) states) = listL states"
+  apply(induction n arbitrary: states)
   by(auto simp: funpow_swap1 invar_step step_listL)
 
 lemmas steps = step_lists Big_Proof.step_list Common_Proof.step_list step_list n_steps
 
 lemmas state_splits = idle.splits Common.state.splits Small.state.splits Big.state.splits
 
-lemma invar_n_steps: "invar transformation \<Longrightarrow> invar ((step^^n) transformation)"
-  apply(induction n arbitrary: transformation)
+lemma invar_n_steps: "invar states \<Longrightarrow> invar ((step^^n) states)"
+  apply(induction n arbitrary: states)
   by(auto simp: invar_step)
 
-lemma step_size_ok: "invar transformation \<Longrightarrow> size_ok transformation \<Longrightarrow> size_ok (step transformation)"
-  apply(induction transformation)
-  apply (metis Transformation.size_ok.simps(1) Transformation.invar.simps(1) Transformation.step.simps(1) prod.case_eq_if prod.exhaust_sel step_size_ok)
-  by (metis Transformation.size_ok.simps(2) Transformation.invar.simps(2) Transformation.step.simps(2) prod.case_eq_if prod.exhaust_sel step_size_ok)
+lemma step_size_ok: "invar states \<Longrightarrow> size_ok states \<Longrightarrow> size_ok (step states)"
+  apply(induction states)
+  apply (metis Transforming.size_ok.simps(1) Transforming.invar.simps(1) Transforming.step.simps(1) prod.case_eq_if prod.exhaust_sel step_size_ok)
+  by (metis Transforming.size_ok.simps(2) Transforming.invar.simps(2) Transforming.step.simps(2) prod.case_eq_if prod.exhaust_sel step_size_ok)
  
-lemma n_steps_size_ok: "invar transformation \<Longrightarrow> size_ok transformation \<Longrightarrow> size_ok ((step ^^ n) transformation)"
+lemma n_steps_size_ok: "invar states \<Longrightarrow> size_ok states \<Longrightarrow> size_ok ((step ^^ n) states)"
   apply(induction n)
    apply(auto simp: funpow_swap1 invar_n_steps step_size_ok)
   by (metis step_size_ok funpow_swap1 invar_n_steps)
 
-lemma remaining_steps_decline_3: "invar transformation \<Longrightarrow> Suc n < remaining_steps transformation
-   \<Longrightarrow> n < remaining_steps (step transformation)"
-proof(induction transformation)
+lemma remaining_steps_decline_3: "invar states \<Longrightarrow> Suc n < remaining_steps states
+   \<Longrightarrow> n < remaining_steps (step states)"
+proof(induction states)
   case (Left small big)
   then show ?case using remaining_steps_decline_3[of "(big, small)" n] 
     by(auto split: prod.splits)
@@ -110,13 +110,13 @@ case (Right big small)
     by(auto split: prod.splits)
 qed
 
-lemma remaining_steps_decline_4: "invar transformation \<Longrightarrow> Suc n < remaining_steps ((step ^^ m) transformation)
-   \<Longrightarrow> n < remaining_steps ((step ^^ Suc m) transformation)"
+lemma remaining_steps_decline_4: "invar states \<Longrightarrow> Suc n < remaining_steps ((step ^^ m) states)
+   \<Longrightarrow> n < remaining_steps ((step ^^ Suc m) states)"
   by(auto simp: remaining_steps_decline_3 invar_n_steps)
 
-lemma remaining_steps_decline_5': "invar transformation \<Longrightarrow> remaining_steps transformation = 1
-   \<Longrightarrow> remaining_steps (step transformation) = 0"
-proof(induction transformation)
+lemma remaining_steps_decline_5': "invar states \<Longrightarrow> remaining_steps states = 1
+   \<Longrightarrow> remaining_steps (step states) = 0"
+proof(induction states)
   case (Left small big)
   then show ?case using remaining_steps_decline_2[of "(big, small)"]
     by(auto split: prod.splits)
@@ -133,7 +133,7 @@ proof(induction n arbitrary: big small)
 next
   case (Suc n)
   then show ?case apply(auto split: prod.splits)
-    by (metis Transformation.step.simps(1) case_prod_unfold funpow_swap1 prod.exhaust_sel) 
+    by (metis Transforming.step.simps(1) case_prod_unfold funpow_swap1 prod.exhaust_sel) 
 qed
 
 lemma remaining_steps_states_remaining_steps_right: "States.remaining_steps ((States.step ^^ n) (big, small)) = remaining_steps ((step ^^ n) (Right big small))"
@@ -143,12 +143,12 @@ proof(induction n arbitrary: big small)
 next
   case (Suc n)
   then show ?case apply(auto split: prod.splits)
-    by (metis Transformation.step.simps(2) case_prod_unfold funpow_swap1 prod.exhaust_sel) 
+    by (metis Transforming.step.simps(2) case_prod_unfold funpow_swap1 prod.exhaust_sel) 
 qed
 
-lemma remaining_steps_decline_5: "invar transformation \<Longrightarrow> remaining_steps transformation \<le> n
-  \<Longrightarrow> remaining_steps ((step ^^ n) transformation) = 0"
-proof(induction transformation)
+lemma remaining_steps_decline_5: "invar states \<Longrightarrow> remaining_steps states \<le> n
+  \<Longrightarrow> remaining_steps ((step ^^ n) states) = 0"
+proof(induction states)
   case (Left small big)
   then show ?case using remaining_steps_decline_5[of "(big, small)" n]
     by(auto simp: remaining_steps_states_remaining_steps_left split: prod.splits)
@@ -159,37 +159,37 @@ next
 qed
 
 
-lemma remaining_steps_step_n: "invar transformation \<Longrightarrow>  n < remaining_steps transformation
-   \<Longrightarrow> remaining_steps transformation - n = remaining_steps ((step ^^ n) transformation)"
-proof(induction transformation)
+lemma remaining_steps_step_n: "invar states \<Longrightarrow>  n < remaining_steps states
+   \<Longrightarrow> remaining_steps states - n = remaining_steps ((step ^^ n) states)"
+proof(induction states)
   case (Left small big)
   then show ?case 
     using remaining_steps_step_n[of "(big, small)" n]
-    by (metis Transformation.invar.simps(1) Transformation.remaining_steps.simps(1) remaining_steps_states_remaining_steps_left)
+    by (metis Transforming.invar.simps(1) Transforming.remaining_steps.simps(1) remaining_steps_states_remaining_steps_left)
 next
   case (Right big small)
   then show ?case
-    by (metis Transformation.invar.simps(2) remaining_steps_step_n funpow_0 remaining_steps_states_remaining_steps_right)
+    by (metis Transforming.invar.simps(2) remaining_steps_step_n funpow_0 remaining_steps_states_remaining_steps_right)
 qed
 
-lemma step_size_ok': "invar transformation \<Longrightarrow>
-    size_ok' transformation x \<Longrightarrow> 
-    size_ok' (step transformation) x"
-proof(induction transformation)
+lemma step_size_ok': "invar states \<Longrightarrow>
+    size_ok' states x \<Longrightarrow> 
+    size_ok' (step states) x"
+proof(induction states)
   case (Left small big)
   then show ?case
-    by (smt (verit, best) States.size_ok'.elims(2) States.size_ok'.elims(3) Transformation.size_ok'.simps(1) Transformation.invar.simps(1) Transformation.step.simps(1) invar_step case_prodE2 case_prod_conv step_size_big step_size_new_small step_size_new_big step_size_small)
+    by (smt (verit, best) States.size_ok'.elims(2) States.size_ok'.elims(3) Transforming.size_ok'.simps(1) Transforming.invar.simps(1) Transforming.step.simps(1) invar_step case_prodE2 case_prod_conv step_size_big step_size_new_small step_size_new_big step_size_small)
 next
   case (Right big small)
   then show ?case 
     using step_size_ok'
-    by (smt (verit, ccfv_threshold) Transformation.size_ok'.simps(2) Transformation.invar.simps(2) Transformation.step.simps(2) invar_step case_prodE2 case_prod_unfold fst_conv snd_conv step_size_ok')
+    by (smt (verit, ccfv_threshold) Transforming.size_ok'.simps(2) Transforming.invar.simps(2) Transforming.step.simps(2) invar_step case_prodE2 case_prod_unfold fst_conv snd_conv step_size_ok')
 qed
 
-lemma step_n_size_ok': "invar transformation \<Longrightarrow>
-    size_ok' transformation x \<Longrightarrow> 
-    size_ok' ((step ^^ n) transformation) x"
-proof(induction n arbitrary: transformation)
+lemma step_n_size_ok': "invar states \<Longrightarrow>
+    size_ok' states x \<Longrightarrow> 
+    size_ok' ((step ^^ n) states) x"
+proof(induction n arbitrary: states)
   case 0
   then show ?case by auto
 next
@@ -198,14 +198,14 @@ next
     by (metis invar_step comp_eq_dest_lhs funpow_Suc_right) 
 qed
 
-lemma size_ok_steps: "invar transformation \<Longrightarrow>
-     n < remaining_steps transformation \<Longrightarrow> 
-    size_ok' transformation (remaining_steps transformation - n) \<Longrightarrow> 
-    size_ok' ((step ^^ n) transformation) (remaining_steps ((step ^^ n) transformation))"
+lemma size_ok_steps: "invar states \<Longrightarrow>
+     n < remaining_steps states \<Longrightarrow> 
+    size_ok' states (remaining_steps states - n) \<Longrightarrow> 
+    size_ok' ((step ^^ n) states) (remaining_steps ((step ^^ n) states))"
   by (simp add: remaining_steps_step_n step_n_size_ok')
 
-lemma size_ok'_size_ok: "size_ok' transformation (remaining_steps transformation) = size_ok transformation"
-  apply(induction transformation rule: size_ok.induct)
+lemma size_ok'_size_ok: "size_ok' states (remaining_steps states) = size_ok states"
+  apply(induction states rule: size_ok.induct)
   by auto
 
 lemma step_n_left_size_new_small: "invar (Left left right) \<Longrightarrow> (step ^^ n) (Left left right) = Left left' right'
